# Design Pattern core concepts ontology
# This document defines and provides the vocabulary to talk about common design pattern elements and their relations
# Many aspects of design patterns can be descibed using existing vocabularies eg dublin core - and where suitable we prefer to use these terms directly rather than invent 
# new subclasses of them here
# This document therefore only covers the intrinsic core pattern elements, and is intended to be extsnsible and evolvable, and to describe design patterns independent of thier 
# specific subject domains.  

# I have copied the layout and many ideas here from the BBC food ontology - http://www.bbc.co.uk/ontologies/fo
# made by Rija Menage, Oliver Bartlett, Philip Lamond, Andrew Robinson and Rob Styles - thanks folks for the inspiration


@base <http://purl.org/ontology/lp/> .

@prefix lp: <<http://purl.org/ontology/lp/> .

# @prefix dcmit: <http://purl.org/dc/dcmitype/> .
@prefix dcterms: <http://purl.org/dc/terms/> .
# @prefix dctypes: <http://purl.org/dc/dcmitype/> .
@prefix foaf: <http://xmlns.com/foaf/0.1/> .
@prefix owl: <http://www.w3.org/2002/07/owl#> .
@prefix rdf: <http://www.w3.org/1999/02/22-rdf-syntax-ns#> .
@prefix rdfs: <http://www.w3.org/2000/01/rdf-schema#> .
# @prefix skos: <http://www.w3.org/2004/02/skos/core#> .
# @prefix v: <http://rdf.data-vocabulary.org/#> .  # << replaced by schema.org?
# @prefix vs: <http://www.w3.org/2003/06/sw-vocab-status/ns#> .
@prefix xsd: <http://www.w3.org/2001/XMLSchema#> .
# @prefix dc:      <http://purl.org/dc/elements/1.1/> .
@prefix po: <http://www.ontologydesignpatterns.org/cp/owl/partof.owl#> .

# @prefix provenance:  <http://www.bbc.co.uk/ontologies/provenance/> .


###################################
# General Schema Info
###################################

lp:
	a owl:Ontology ;
	dcterms:title "Design Pattern Core Ontology"@en ;
	rdfs:label "Design Pattern Core Ontology"^^xsd:string ;
	rdfs:comment "A simple vocabulary for describing design patterns."@en ;
	foaf:maker <#cam> ;
	dcterms:created "2014-04-30"^^xsd:date ;
	dcterms:license <http://creativecommons.org/licenses/by/4.0#id> ;
#	provenance:canonicalLocation
#              "https://wherever.it.ends.up/lp.ttl"^^xsd:string ;
#   provenance:version "1.0"^^xsd:double ;
#   provenance:public "true"^^xsd:boolean ;
#   owl:imports vs: , dc: , dcterms: , foaf: , provenance: ;      <<<<<<<<<<< which ontologies do I need to import fully??
 	owl:imports po: ;.
#    owl:versionIRI <http://purl.org/ontology/lp/1.0> ;
#    owl:versionInfo "1.0"^^xsd:string .


<#cam> a foaf:Person ;
	foaf:name "Cameron McLean" .


###################################
#  Classes
###################################

lp:DesignPattern a owl:Class ;
	rdfs:label "Design Patten"@en ;
	rdfs:comment "A design pattern is a... "@en ;
	po:hasPart lp:Force ;
	po:hasPart lp:Problem ;
	po:hasPart lp:Context ;
	po:hasPart lp:Solution ;
	po:hasPart lp:Rationale ;
	po:hasPart lp:Pictogram ;
	rdfs:isDefinedBy lp: .

lp:Force a owl:Class ;
	po:partOf lp:DesignPattern ;
	rdfs:label "Force"@en ;
	rdfs:comment "A 'force' is the term used to describe things ... "@en ;
	rdfs:isDefinedBy lp: .

lp:Problem a owl:Class ;
	po:partOf lp:DesignPattern ;
	rdfs:label "Problem"@en ;
	rdfs:comment "A problem describes ...."@en ;
	rdfs:isDefinedBy lp: .

lp:Context a owl:Class ;
	po:partOf lp:DesignPattern ;
	rdfs:label "Context"@en ;
	rdfs:comment "The context describes things ... "@en ;
	rdfs:isDefinedBy lp: .

lp:Solution a owl:Class ;
	po:partOf lp:DesignPattern ;
	rdfs:label "Solution"@en ;
	rdfs:comment "The solution describes things ... "@en ;
	rdfs:isDefinedBy lp: .

lp:Rationale a owl:Class ;
	po:partOf lp:DesignPattern ;
	rdfs:label "Rationale"@en ;
	rdfs:comment "The rationale describes things ... "@en ;
	rdfs:isDefinedBy lp: .

lp:Pictogram a owl:Class ;
	po:partOf lp:DesignPattern ;
	po:partOf lp:Force ;
	rdfs:label "Pictogram"@en ;
	rdfs:comment "A pictogram provides a visual depiction of ..."@en ;
	rdfs:isDefinedBy lp: .

lp:Reference a owl:Class ;
	po:PartOf lp:DesignPattern ;
	rdfs:label "Reference"@en ;
	rdfs:comment "A reference is the biliographic entity that supplies the justification for a solution and its rationale ..." ;
	rdfs:isDefinedBy lp: .


###################################
#  Object Properties
###################################

# Pattern Relationships

lp:uses a owl:ObjectProperty ;
	rdfs:label "uses"@en ;
	rdfs:comment "The 'uses' property relates a design pattern to another pattern that it uses in its solution"@en ;
	rdfs:range lp:DesignPattern ;
	rdfs:domain lp:DesignPattern ;
	owl:inverseOf lp:UsedBy ;
	rdfs:isDefinedBy lp: .

lp:usedBy a owl:ObjectProperty ;
	rdfs:label "used by"@en ;
	rdfs:comment "The 'usedBy' property relates a design pattern to another pattern that uses it in its solution"@en ;
	rdfs:range lp:DesignPattern ;
	rdfs:domain lp:DesignPattern ;
	owl:inverseOf lp:uses ;
	rdfs:isDefinedBy lp: .

lp:upstreamOf a owl:ObjectProperty ;
	rdfs:label "upstream of"@en ;
	rdfs:comment "The 'upstreamOf' property relates a design pattern to smaller, more specific/granualar, or other patterns that might be considered after applying this one"@en ;
	rdfs:range lp:DesignPattern ;
	rdfs:domain lp:DesignPattern ;
	owl:inverseOf lp:downstreamOf ;
	rdfs:isDefinedBy lp: .

lp:downstreamOf a owl:ObjectProperty ;
	rdfs:label "downstream of"@en ;
	rdfs:comment "The 'downstreamOf' property relates a design pattern to larger, more general/abstract, or other patterns that might be considered before applying this one"@en ;
	rdfs:range lp:DesignPattern ;
	rdfs:domain lp:DesignPattern ;
	owl:inverseOf lp:upstreamOf ;
	rdfs:isDefinedBy lp: .

lp:relatedTo a owl:ObjectProperty ;
	rdfs:label "related to"@en ;
	rdfs:comment "The 'related' property provides a generic way of linking patterns that might be similar, relevent, alternative, or otherwise of interest"@en ;
	rdfs:range lp:DesignPattern ;
	rdfs:domain lp:DesignPattern ;
	rdfs:isDefinedBy lp: .

lp:incompatibleWith a owl:ObjectProperty ;
	rdfs:label "incompatible with"@en ;
	rdfs:comment "The 'incompatible' property relates design patterns that cannont be used together in the same larger sequence. Use of one will prevent the use of another."@en ;
	rdfs:range lp:DesignPattern ;
	rdfs:domain lp:DesignPattern ;
	rdfs:isDefinedBy lp: .


# Relationships between pattern/force and external resources

lp:exemplifiedBy a owl:ObjectProperty ;
	rdfs:label "exemplified by"@en ;
	rdfs:comment "The 'exemplified by' property is used to relate an overall pattern or a force to other resources that are instances of pattern occurances or solutions to forces in the real world"@en ;
	rdfs:isDefinedBy lp: .


###################################
#  Datatype Properties
###################################

