<?xml version="1.0" encoding="UTF-8"?>
<rdf:RDF
   xmlns:core="http://vivoweb.org/ontology/core#"
   xmlns:dcterms="http://purl.org/dc/terms/"
   xmlns:foaf="http://xmlns.com/foaf/0.1/"
   xmlns:rdf="http://www.w3.org/1999/02/22-rdf-syntax-ns#"
   xmlns:rdfs="http://www.w3.org/2000/01/rdf-schema#"
>
  <rdf:Description rdf:about="http://purl.org/NET/labpatterns#Force">
    <rdf:type rdf:resource="http://www.w3.org/2002/07/owl#Class"/>
    <rdfs:label xml:lang="en">Force</rdfs:label>
    <dcterms:partOf rdf:resource="http://purl.org/NET/labpatterns#DesignPattern"/>
    <rdfs:comment xml:lang="en">A 'force' is the term used to describe constraints imposed by a pattern context that shape both the problem and how it should be solved.</rdfs:comment>
    <rdfs:isDefinedBy rdf:resource="http://purl.org/NET/labpatterns#"/>
  </rdf:Description>
  <rdf:Description rdf:about="http://purl.org/NET/labpatterns#hasRationale">
    <rdfs:range rdf:resource="http://www.w3.org/2001/XMLSchema#string"/>
    <rdfs:domain rdf:resource="http://purl.org/NET/labpatterns#DesignPattern"/>
    <rdfs:label xml:lang="en">rationale</rdfs:label>
    <rdf:type rdf:resource="http://www.w3.org/2002/07/owl#DatatypeProperty"/>
    <rdfs:comment xml:lang="en">The rationale describes the evidence and reasoning as to why the problem/forces exist and why the solution works.</rdfs:comment>
    <rdfs:isDefinedBy rdf:resource="http://purl.org/NET/labpatterns#"/>
  </rdf:Description>
  <rdf:Description rdf:about="http://purl.org/NET/labpatterns#cam">
    <foaf:name>Cameron McLean</foaf:name>
    <core:orcidId rdf:resource="http://orcid.org/0000-0002-9836-3824"/>
    <foaf:homepage rdf:resource="http://cameronmclean.github.io"/>
    <rdf:type rdf:resource="http://xmlns.com/foaf/0.1/Person"/>
  </rdf:Description>
  <rdf:Description rdf:about="http://purl.org/NET/labpatterns#">
    <rdfs:label rdf:datatype="http://www.w3.org/2001/XMLSchema#string">Design Pattern Core Ontology</rdfs:label>
    <dcterms:title xml:lang="en">Design Pattern Core Ontology</dcterms:title>
    <dcterms:created rdf:datatype="http://www.w3.org/2001/XMLSchema#date">2015-03-10</dcterms:created>
    <rdfs:comment xml:lang="en">A simple vocabulary for describing design patterns.</rdfs:comment>
    <dcterms:license rdf:resource="http://creativecommons.org/licenses/by/4.0#id"/>
    <rdf:type rdf:resource="http://www.w3.org/2002/07/owl#Ontology"/>
    <foaf:maker rdf:resource="http://purl.org/NET/labpatterns#cam"/>
  </rdf:Description>
  <rdf:Description rdf:about="http://purl.org/NET/labpatterns#Reference">
    <rdfs:comment xml:lang="en">A bibliographic record that contains evidence of design pattern concepts or rationale.</rdfs:comment>
    <rdfs:isDefinedBy rdf:resource="http://purl.org/NET/labpatterns#"/>
    <rdf:type rdf:resource="http://www.w3.org/2002/07/owl#Class"/>
    <rdfs:label xml:lang="en">Reference</rdfs:label>
    <dcterms:partOf rdf:resource="http://purl.org/NET/labpatterns#DesignPattern"/>
  </rdf:Description>
  <rdf:Description rdf:about="http://purl.org/NET/labpatterns#DesignPattern">
    <rdf:type rdf:resource="http://www.w3.org/2002/07/owl#Class"/>
    <rdfs:comment xml:lang="en">A design pattern is a structured description that captures expert knowledge and solutions to recurring problems enabling the generalisation and communication of design knowledge.</rdfs:comment>
    <rdfs:label xml:lang="en">Design Patten</rdfs:label>
    <rdfs:isDefinedBy rdf:resource="http://purl.org/NET/labpatterns#"/>
  </rdf:Description>
  <rdf:Description rdf:about="http://purl.org/NET/labpatterns#hasSolution">
    <rdfs:domain rdf:resource="http://purl.org/NET/labpatterns#DesignPattern"/>
    <rdf:type rdf:resource="http://www.w3.org/2002/07/owl#DatatypeProperty"/>
    <rdfs:range rdf:resource="http://www.w3.org/2001/XMLSchema#string"/>
    <rdfs:comment xml:lang="en">The solution describes how to resolve the forces that create the problem.</rdfs:comment>
    <rdfs:isDefinedBy rdf:resource="http://purl.org/NET/labpatterns#"/>
    <rdfs:label xml:lang="en">solution</rdfs:label>
  </rdf:Description>
  <rdf:Description rdf:about="http://purl.org/NET/labpatterns#Contributor">
    <rdf:type rdf:resource="http://xmlns.com/foaf/0.1/Person"/>
    <rdfs:label xml:lang="en">Contributor</rdfs:label>
    <rdf:type rdf:resource="http://www.w3.org/2002/07/owl#Class"/>
    <rdfs:comment xml:lang="en">An identifier and reference to a person who creates or edits design patterns.</rdfs:comment>
    <rdfs:isDefinedBy rdf:resource="http://purl.org/NET/labpatterns#"/>
  </rdf:Description>
  <rdf:Description rdf:about="http://purl.org/NET/labpatterns#hasForce">
    <rdfs:domain rdf:resource="http://purl.org/NET/labpatterns#DesignPattern"/>
    <rdf:type rdf:resource="http://www.w3.org/2002/07/owl#ObjectProperty"/>
    <rdfs:isDefinedBy rdf:resource="http://purl.org/NET/labpatterns#"/>
    <rdfs:range rdf:resource="http://purl.org/NET/labpatterns#Force"/>
    <rdfs:comment xml:lang="en">Relates a named Force to it's parent/specific design pattern.</rdfs:comment>
    <rdfs:label xml:lang="en">force</rdfs:label>
  </rdf:Description>
  <rdf:Description rdf:about="http://purl.org/NET/labpatterns#hasProblem">
    <rdf:type rdf:resource="http://www.w3.org/2002/07/owl#DatatypeProperty"/>
    <rdfs:label xml:lang="en">problem</rdfs:label>
    <rdfs:comment xml:lang="en">The problem is concise statement that summarises the situation that the pattern resolves.</rdfs:comment>
    <rdfs:range rdf:resource="http://www.w3.org/2001/XMLSchema#string"/>
    <rdfs:isDefinedBy rdf:resource="http://purl.org/NET/labpatterns#"/>
    <rdfs:domain rdf:resource="http://purl.org/NET/labpatterns#DesignPattern"/>
  </rdf:Description>
  <rdf:Description rdf:about="http://purl.org/NET/labpatterns#hasContext">
    <rdf:type rdf:resource="http://www.w3.org/2002/07/owl#DatatypeProperty"/>
    <rdfs:range rdf:resource="http://www.w3.org/2001/XMLSchema#string"/>
    <rdfs:label xml:lang="en">context</rdfs:label>
    <rdfs:isDefinedBy rdf:resource="http://purl.org/NET/labpatterns#"/>
    <rdfs:comment xml:lang="en">The context describes the original configuration of the system in which the problem occurs.</rdfs:comment>
    <rdfs:domain rdf:resource="http://purl.org/NET/labpatterns#DesignPattern"/>
  </rdf:Description>
</rdf:RDF>

